Optimizations/Canonicalizations/AddPhase.thy
@@ -36,14 +36,19 @@ optimization AddNeutral: "(e + (const (IntVal32 0))) \<mapsto> e"
   unfolding rewrite_preservation.simps
   sorry
 
-optimization NeutralLeftSub: "(e\<^sub>1 - e\<^sub>2) + e\<^sub>2 \<mapsto> e\<^sub>1"
+ML_val \<open>@{term \<open>x = y\<close>}\<close>
+
+optimization NeutralLeftSub[intval]: "((e\<^sub>1 - e\<^sub>2) + e\<^sub>2) \<mapsto> e\<^sub>1"
   unfolding rewrite_preservation.simps rewrite_termination.simps
-   apply (rule conjE, simp, simp del: le_expr_def)
+    apply (rule conjE, simp; simp del: le_expr_def) unfolding intval.simps
+  using intval_add.simps intval_sub.simps
+    apply (metis (no_types, lifting) diff_add_cancel val_to_bool.cases)
   sorry
 
-optimization NeutralRightSub: " e\<^sub>2 + (e\<^sub>1 - e\<^sub>2) \<mapsto> e\<^sub>1"
+optimization NeutralRightSub[intval]: " e\<^sub>2 + (e\<^sub>1 - e\<^sub>2) \<mapsto> e\<^sub>1"
   unfolding rewrite_preservation.simps rewrite_termination.simps
-   apply (rule conjE, simp, simp del: le_expr_def)
+    apply (rule conjE, simp, simp del: le_expr_def)
+  using NeutralLeftSub(1) intval_add_sym apply auto[1]
   sorry
 
 optimization AddToSub: "-e + y \<mapsto> y - e"
